%! Author = Johannes Byle
%! Date = 8/29/2021

% Preamble
\documentclass[12pt]{article}
\title{Quantum I Assignment \#1}
\author{Johannes Byle}
\newcommand{\op}[1]{\tilde{\mathbf{#1}}}

% Packages
\usepackage{amsmath}
\usepackage[margin=0.75in]{geometry}
\usepackage{lipsum}
\usepackage{braket}

% Document
\begin{document}
    \maketitle
    \begin{enumerate}
        \item[Q-1]
        \begin{enumerate}
            \item $\op{K}$ is hermitian iff:
            \[
                \op{K}=\op{K}^{\dagger}
            \]
            \item
            \begin{gather*}
                \op{K}=\ket{\phi}\bra{\psi}\\
                \op{K}^2=\left(\ket{\phi}\bra{\psi}\right)\left(\ket{\phi}\bra{\psi}\right)
            \end{gather*}
            Because of the associative principle:
            \begin{gather*}
                \op{K}^2=\ket{\phi}\braket{\psi|\phi}\bra{\psi}
            \end{gather*}
            $\op{K}^2$ is a projection operator if $\psi=\phi$
            \begin{gather*}
                \op{K}^2=\ket{\psi}\braket{\psi|\psi}\bra{\psi}\\
                \op{K}^2=\ket{\psi}1\bra{\psi}\\
                \op{K}^2=\ket{\psi}\bra{\psi}
            \end{gather*}
            \item
            Assuming $\op{P}_1=\ket{\phi}\bra{\phi}$ and $\op{P}_2=\ket{\psi}\bra{\psi}$
            \begin{gather*}
                \op{K}=\lambda\ket{\phi}\braket{\phi|\psi}\bra{\psi}
            \end{gather*}
            From equation 1.25 we know that the product of $\braket{\phi|\psi}$ is normally a complex number, therefore, assuming scalar multiplication with vectors is commutative:
            \begin{gather*}
                \braket{\phi|\psi}=c\\
                \op{K}=\lambda\ket{\phi}c\bra{\psi}\\
                \op{K}=\lambda\ket{\phi}\bra{\psi}\quad\text{We can just combine $c$ into $\lambda$}
            \end{gather*}
        \end{enumerate}
        \item[1.1]
        Assumptions:
        \begin{gather*}
            v_{th}=\sqrt{\frac{2k_b T}{m}}\\
            t=\frac{\Delta x}{v_{th}}\\
            F_z=ma_z=\mu_z\frac{\delta B_z}{\delta z}\\
            \Delta z=\frac{1}{2}a_z t^2
        \end{gather*}
        Substituting variables:
        \begin{gather*}
            \Delta z=\frac{1}{2}\mu_z\frac{\delta B_z}{\delta z}\frac{1}{m}\frac{\sqrt{\Delta x}}{2k_b T}m\\
            \Delta z=\mu_z\frac{\delta B_z}{\delta z}\frac{\sqrt{\Delta x}}{4k_b T}\\
            \Delta z=9.27\cdot10^{-24}\cdot10\cdot\frac{1}{4\cdot1.38\cdot10^{-23}\cdot1273.15}\approx0.0013\text{ m}
        \end{gather*}
        \item[1.3]
        \begin{gather*}
            \braket{(\Delta A)^2}\braket{(\Delta B)^2}\geq\frac{1}{4}\left|\braket{\left[A,B\right]}\right|^2
        \end{gather*}
        For $A=S_x$ and $B=S_y$:
        \begin{gather*}
            \braket{(\Delta S_x)^2}\braket{(\Delta S_y)^2}\geq\frac{1}{4}\left|\braket{\left[S_x,S_y\right]}\right|^2\\
            \left(\braket{S_x^2}-\braket{S_x}^2\right)\left(\braket{S_y^2}-\braket{S_y}^2\right)\geq\frac{1}{4}\left|i\hbar S_z\right|^2\\
            \left(0\right)
            \left(\frac{\hbar}{2}\right)
            \geq\frac{1}{4}\left|i\hbar S_z\right|^2\\
            0\geq\frac{1}{4}\left|i\hbar \braket{S_y ;\pm|S_x ;+}\right|^2\\
            0\geq\frac{1}{4}\left|i\hbar \frac{1}{\sqrt{2}}\right|^2\\
            0\geq-\frac{\hbar^2}{16}
        \end{gather*}
        For $A=S_z$ and $B=S_y$:
        \begin{gather*}
            \braket{(\Delta S_z)^2}\braket{(\Delta S_y)^2}\geq\frac{1}{4}\left|\braket{\left[S_z,S_y\right]}\right|^2\\
            \left(\braket{S_z^2}-\braket{S_z}^2\right)\left(\braket{S_y^2}-\braket{S_y}^2\right)\geq\frac{1}{4}\left|i\hbar S_x\right|^2\\
            \left(\frac{\hbar}{2}\right)
            \left(\frac{\hbar}{2}\right)
            \geq\frac{1}{4}\left|i\hbar S_z\right|^2\\
            \frac{\hbar^2}{4}\geq\frac{1}{4}\left|i\hbar \braket{S_x ;\pm|S_x ;+}\right|^2\\
            \frac{\hbar^2}{4}\geq\frac{1}{4}\left|i\hbar1\right|^2\\
            \frac{\hbar^2}{4}\geq-\frac{\hbar^2}{4}
        \end{gather*}
        \item[1.7]
        \begin{enumerate}
            \item
            \begin{gather*}
                \begin{bmatrix}
                    \braket{a^{(1)}|\alpha}\braket{\beta|a^{(1)}} & \braket{a^{(1)}|\alpha}\braket{\beta|a^{(2)}} & \ldots\\
                    \braket{a^{(2)}|\alpha}\braket{\beta|a^{(1)}} & \braket{a^{(2)}|\alpha}\braket{\beta|a^{(2)}} & \ldots\\
                    \vdots                                        & \vdots                                        & \ddots
                \end{bmatrix}
            \end{gather*}
            \item
            \begin{gather*}
                \begin{bmatrix}
                    \braket{a^{(1)}|S_z ;+}\braket{S_x ;+|a^{(1)}} & \braket{a^{(1)}|S_z ;+}\braket{S_x ;+|a^{(2)}} \\
                    \braket{a^{(2)}|S_z ;+}\braket{S_x ;+|a^{(1)}} & \braket{a^{(2)}|S_z ;+}\braket{S_x ;+|a^{(2)}}
                \end{bmatrix}\\
                \begin{bmatrix}
                    \frac{\hbar}{2}\cdot0 & 0\cdot\frac{\hbar}{2}  \\
                    0\cdot\frac{\hbar}{2} & -\frac{\hbar}{2}\cdot0
                \end{bmatrix}=
                \begin{bmatrix}
                    0 & 0 \\
                    0 & 0 \\
                \end{bmatrix}
            \end{gather*}
        \end{enumerate}
        \item[1.8]
    \end{enumerate}

\end{document}