%! Author = johannes
%! Date = 9/20/21

% Preamble
\documentclass[12pt]{article}
\title{Quantum I Assignment \#4}
\author{Johannes Byle}
\newcommand{\op}[1]{\tilde{\mathbf{#1}}}

% Packages
\usepackage{amsmath}
\usepackage[margin=0.75in]{geometry}
\usepackage{lipsum}
\usepackage{braket}
\usepackage{hyperref}

% Document
\begin{document}
  \maketitle
  \begin{enumerate}
    \item[1.13]
    Assuming that the observable is $\ket{E}$ with eigenkets $a\ket{1}+b\ket{2}$:
    \begin{gather}
      H\ket{E}=\left(H_{11}\ket{1}\bra{1}+H_{22}\ket{2}\bra{2}+H_{12}[\ket{1}\bra{2}+\ket{2}\bra{1}]\right)(a\ket{1}+b\ket{2})\\
      H\ket{E}=H_{11}a\ket{1}+H_{22}b\ket{2}+H_{12}b\ket{1}+H_{12}a\ket{2}
    \end{gather}
    Since $H\ket{E}=\lambda\ket{E}=\lambda a\ket{1}+\lambda b\ket{2}$:
    \begin{gather}
      \lambda a=H_{11}a+H_{12}b\\
      \lambda b=H_{22}b+H_{12}a
    \end{gather}
    Using substition to solve for $\lambda$:
    \begin{gather}
      \frac{\lambda(a-H_{11})}{H_{12}}=b\\
      \frac{\lambda(a-H_{11})}{H_{12}}(\lambda-H_{22})=H_{12}a
    \end{gather}
    \item[1.18]
    If $\ket{\psi}$ is a eigenket of both $A$ and $B$ then:
    \begin{gather*}
      A\ket{\psi}=a\ket{\psi}\\
      B\ket{\psi}=b\ket{\psi}\\
      (AB+BA)\ket{\psi}=2ab\ket{\psi}
    \end{gather*}
    The only way this is true is if either $a$ or $b$ is 0.\footnote{http://peeterjoot.com/2015/09/28/can-anticommuting-operators-have-a-simulaneous-eigenket/}
    \item[1.25]
    \begin{enumerate}
      \item No:
      \begin{gather}
        \begin{bmatrix}
          b & 0  & 0   \\
          0 & 0  & -ib \\
          0 & ib & 0
        \end{bmatrix}
        \begin{bmatrix}
          1 \\
          0 \\
          0
        \end{bmatrix}=b\\
        \begin{bmatrix}
          b & 0  & 0   \\
          0 & 0  & -ib \\
          0 & ib & 0
        \end{bmatrix}
        \begin{bmatrix}
          0 \\
          1 \\
          0
        \end{bmatrix}=-ib\\
        \begin{bmatrix}
          b & 0  & 0   \\
          0 & 0  & -ib \\
          0 & ib & 0
        \end{bmatrix}
        \begin{bmatrix}
          0 \\
          0 \\
          1
        \end{bmatrix}=ib
      \end{gather}
      \item
      \begin{gather}
        \begin{bmatrix}
          a & 0  & 0  \\
          0 & -a & 0  \\
          0 & 0  & -a
        \end{bmatrix}
        \begin{bmatrix}
          b & 0  & 0   \\
          0 & 0  & -ib \\
          0 & ib & 0
        \end{bmatrix}=
        \begin{bmatrix}
          ab & 0    & 0   \\
          0  & 0    & iab \\
          0  & -iab & 0
        \end{bmatrix}\\
        \begin{bmatrix}
          b & 0  & 0   \\
          0 & 0  & -ib \\
          0 & ib & 0
        \end{bmatrix}
        \begin{bmatrix}
          a & 0  & 0  \\
          0 & -a & 0  \\
          0 & 0  & -a
        \end{bmatrix}=
        \begin{bmatrix}
          ab & 0    & 0   \\
          0  & 0    & iab \\
          0  & -iab & 0
        \end{bmatrix}
      \end{gather}
    \end{enumerate}
  \end{enumerate}

\end{document}