%! Author = johannes
%! Date = 9/20/21

% Preamble
\documentclass[12pt]{article}
\title{Quantum I Assignment \#5}
\author{Johannes Byle}
\newcommand{\op}[1]{\tilde{\mathbf{#1}}}

% Packages
\usepackage{amsmath}
\usepackage[margin=0.75in]{geometry}
\usepackage{lipsum}
\usepackage{braket}
\usepackage{mathrsfs}
\newcommand{\opx}{\pmb{\text{x}}}
\newcommand{\jac}{\mathscr{J}(d\opx')}
\newcommand{\jacdag}{\mathscr{J}^{\dag}(d\opx')}
\newcommand{\opp}{\pmb{\text{p}}}
\newcommand{\boost}{\mathscr{B}(d\opp')}
\newcommand{\boostdag}{\mathscr{B}^{\dag}(d\opp')}
\newcommand{\opw}{\pmb{\text{W}}}
\newcommand{\p}[2]{\frac{\partial #1}{\partial #2}}
% Document
\begin{document}
  \maketitle
  \begin{enumerate}
    \item[Q-1]
    \begin{align*}
    [\op{X},\op{H}]
    \end{align*}
    \item[1.33] Starting with the translation operator applied to the expectation value for $\opx$:
    \begin{gather*}
      \bra{\alpha}\jacdag\opx\jac\ket{\alpha}\\
    \end{gather*}
    By equation 1.207 we know:
    \begin{gather*}
      \opx\jac-\jac\opx=d\opx'
    \end{gather*}
    Since the translation operator is unitary we can apply $\jacdag$ to both sides:
    \begin{gather*}
      \jacdag\left[\opx\jac-\jac\opx\right]=\jacdag d\opx'\\
      \jacdag \opx\jac-\jacdag\jac\opx=\jacdag d\opx'\\
      \jacdag \opx\jac-\opx=\jacdag d\opx'\\
      \opx+d\opx'-\opx=\jacdag d\opx'
    \end{gather*}
    This means that $\bra{\alpha}\jacdag\opx\jac\ket{\alpha}\rightarrow\bra{\alpha}\opx\ket{\alpha}+d\opx'$.\\
    Using the same process for $\opp$:
    By equation 1.227 we know:
    \begin{gather*}
      \opp\jac-\jac\opp=0
    \end{gather*}
    Since the translation operator is unitary we can apply $\jacdag$ to both sides:
    \begin{gather*}
      \jacdag\left[\opp\jac-\jac\opp\right]=0\\
      \jacdag \opp\jac-\jacdag\jac\opp=0\\
      \jacdag \opp\jac-\opp=0\\
      \opp+d\opp'-\opp=0
    \end{gather*}
    This means that $\bra{\alpha}\jacdag\opp\jac\ket{\alpha}\rightarrow\bra{\alpha}\opp\ket{\alpha}$.\\
    \item[1.34] Satisfies unitary property because $\opw$ is hermitian:
    \begin{align*}
      \boostdag\boost&=(1-i\opw\cdot d\opp)(1+i\opw\cdot d\opp)\\
      &=(1-i\opw\cdot d\opp^{\dagger})(1+i\opw\cdot d\opp)\\
      &=1-i(\opw-\opw^{\dagger})\\
      &\simeq 1
    \end{align*}
    Satisfies the associative property:
    \begin{align*}
      \boostdag\mathscr{B}(d\opp'')&=(1+i\opw\cdot d\opp')\cdot(1+i\opw\cdot d\opp'')\\
      &\simeq 1-i\opw\cdot(d\opp' d\opp'')\\
      &= \mathscr{B}(d\opp'+d\opp'')
    \end{align*}
    Satisfies the inverse property trivially:
    \begin{align*}
      \mathscr{B}(-d\opp')&=\mathscr{B}^{-1}(d\opp')\\
      1+i\opw\cdot d\opp&=-(-1-i\opw\cdot d\opp)
    \end{align*}
    Since $d\opp$ has units of $\frac{\text{kg m}}{\text{s}^2}$
    \item[1.35]
    \begin{enumerate}
      \item
      \begin{align*}
        \braket{p}&=\int_{-\infty}^{\infty}dx'\braket{\alpha|x'}(-i\hbar\p{}{x'})\braket{x'|\alpha}\\
        &=\int_{-\infty}^{\infty}dx'\left[\frac{1}{\pi^{1/4}\sqrt{d}}\right]\exp\left[-ikx'-\frac{x'^2}{2d^2}\right](-i\hbar\p{}{x'})\left[\frac{1}{\pi^{1/4}\sqrt{d}}\right]\exp\left[ikx'-\frac{x'^2}{2d^2}\right]\\
        &=\left[\frac{-i\hbar}{\pi^{1/2}d}\right]\int_{-\infty}^{\infty}dx'\exp\left[-ikx'-\frac{x'^2}{2d^2}\right]\p{}{x'}\exp\left[ikx'-\frac{x'^2}{2d^2}\right]\\
        &=\left[\frac{-i\hbar}{\pi^{1/2}d}\right]\int_{-\infty}^{\infty}dx'\left[ ik-\frac{x'}{d^2} \right]\exp\left[-\frac{x'^2}{d^2}\right]\\
        &=\left[\frac{-i\hbar}{\pi^{1/2}d}\right]\left(\frac{-k\pi^{1/2}d}{i}\right)\\
        &=\hbar k
      \end{align*}
      \begin{align*}
        \braket{p^2}&=\int_{-\infty}^{\infty}dx'\braket{\alpha|x'}(-i\hbar\p{}{x'})^2\braket{x'|\alpha}\\
        &=\hbar^2\int_{-\infty}^{\infty}dx'\left[\frac{1}{\pi^{1/4}\sqrt{d}}\right]\exp\left[-ikx'-\frac{x'^2}{2d^2}\right]\p{^2}{x'^2}\left[\frac{1}{\pi^{1/4}\sqrt{d}}\right]\exp\left[-ikx'-\frac{x'^2}{2d^2}\right]\\
        &=\frac{\hbar^2}{2d^2}+\hbar^2 k^2
      \end{align*}
      \item
      \begin{align*}
        \braket{p|\alpha}&=\int_{-\infty}^{\infty}dx'\braket{\alpha|x'}(-i\hbar\p{}{x'})\braket{x'|\alpha}\\
        &=\int_{-\infty}^{\infty}dp\sqrt{\frac{d}{\hbar\sqrt{\pi}}}\exp\left[\frac{-(p'-\hbar k)^2 d^2}{2\hbar^2}\right](-i\hbar\p{}{x'})\sqrt{\frac{d}{\hbar\sqrt{\pi}}}\exp\left[\frac{-(p'-\hbar k)^2 d^2}{2\hbar^2}\right]\\
        &=\hbar k
      \end{align*}
      \begin{align*}
        \braket{p^2|\alpha}&=\int_{-\infty}^{\infty}dx'\braket{\alpha|x'}(-i\hbar\p{}{x'})^2\braket{x'|\alpha}\\
        &=\hbar^2\int_{-\infty}^{\infty}dp\sqrt{\frac{d}{\hbar\sqrt{\pi}}}\exp\left[\frac{-(p'-\hbar k)^2 d^2}{2\hbar^2}\right]\p{^2}{x'^2}\sqrt{\frac{d}{\hbar\sqrt{\pi}}}\exp\left[\frac{-(p'-\hbar k)^2 d^2}{2\hbar^2}\right\\
        &=\frac{\hbar^2}{2d^2}+\hbar^2 k^2
      \end{align*}
    \end{enumerate}
    \item[1.36]
    \begin{enumerate}
      \item
      \begin{enumerate}
        \item
        Using equation (1.265a) $\braket{p'|\alpha}=\int dx'\braket{p'|x'}\braket{x'|\alpha}$:
        \begin{align*}
          \braket{p'|x|\alpha}&=\int dx'\braket{p'|x|x'}\braket{x'|\alpha}\\
          &=\int dx'x'\braket{p'|x'}\braket{x'|\alpha}\\
          &=\frac{1}{\sqrt{2\pi\hbar}}\int dx'x'\exp\left[\frac{-ip'x'}{\hbar}\right]\braket{x'|\alpha}\quad\text{using (1.264)}\\
          &=\frac{1}{\sqrt{2\pi\hbar}}\int dx'\p{}{p'}i\hbar\exp\left[\frac{-ip'x'}{\hbar}\right]\braket{x'|\alpha}\\
          &=i\hbar\p{}{p'}\int dx'\frac{1}{\sqrt{2\pi\hbar}}\exp\left[\frac{-ip'x'}{\hbar}\right]\braket{x'|\alpha}=i\hbar\p{}{p'}\braket{p'|\alpha}\\
          \braket{p'|x|\alpha}&=i\hbar\p{}{p'}\braket{p'|\alpha}\
        \end{align*}
        \item This holds true from the previous result:
        \begin{align*}
          \braket{\beta|x|\alpha}&=\int dp'\braket{\beta|p'}\braket{p'|x|\alpha}=\int dp'x\braket{\beta|p'}\braket{p'\alpha}\\
          &=\int dp'\braket{\beta|p'}i\hbar\p{}{p'}\braket{p'\alpha}\quad\text{from the previous part}\\
          \braket{\beta|x|\alpha}&=\int dp'\phi_{\beta}(p')i\hbar\p{}{p'}\phi_{\alpha}(p')\\
        \end{align*}
      \end{enumerate}
      \item
    \end{enumerate}
  \end{enumerate}


\end{document}