%! Author = johannes
%! Date = 11/2/21

% Preamble
\documentclass[10pt]{article}
\title{Quantum I Assignment \#8}
\author{Johannes Byle}


% Packages
\usepackage{amsmath}
\usepackage[margin=0.75in]{geometry}
\usepackage{lipsum}
\usepackage{physics}
\usepackage{bbold}
\usepackage{braket}
\newcommand{\p}[2]{\frac{\partial #1}{\partial #2}}
\newcommand{\der}[2]{\frac{d #1}{d #2}}
\newcommand{\OP}[1]{\tilde{\pmb{\text{#1}}}}
\newcommand{\Fop}[1]{\mathcal{#1}}

% Document
\begin{document}
  \maketitle
  \begin{enumerate}
    \item
    \begin{enumerate}
      \item Since $\psi(x,0)$ must be normalized:
      \begin{gather*}
        \int_{-\infty}^{\infty}\psi(x,0)dx=\frac{\sqrt{\pi } A \left(\sin (\beta )+\sqrt{2} \cos (\beta )\right)}{\sqrt{\alpha ^2}}=1\\
        A=-\frac{\sqrt{\alpha ^2}}{\sqrt{\pi } (-\sin (\beta ))+\left(-\sqrt{2 \pi }\right) \cos (\beta )}
      \end{gather*}
      \item Since $E_n=(n+\frac{1}{2})\hbar\omega$:
      \begin{gather*}
        E=\frac{1}{2}\hbar\omega,\ \frac{5}{2}\hbar\omega
      \end{gather*}
      \item
      \begin{gather*}
        \int\psi(x,0)x\psi(x,0)=\frac{A^2 e^{\alpha ^2 \left(-x^2\right)} \left(2 \sqrt{2} \sin (2 \beta ) \left(2 \alpha ^2 x^2+1\right)-\cos (2 \beta ) \left(4 \alpha ^4 x^4+4 \alpha ^2 x^2+3\right)+4 \alpha ^4 x^4+4 \alpha ^2 x^2+7\right)}{8 \alpha ^2}\\
        \int_{-\infty}^{\infty}\psi(x,0)x\psi(x,0)=0
      \end{gather*}
    \end{enumerate}
    \item[2.15]\footnote{https://www3.nd.edu/~bjanko/p70007/qm1hw4answers.pdf}
    \begin{enumerate}
      \item Since $\psi(x)=\braket{x|e^{\frac{-ipa}{\hbar}}|0}$ which is the spatial translation operator where $e^{\frac{-ipa}{\hbar}}\ket{x}=\ket{x+a}$:
      \begin{gather*}
        \psi(x)=\int\braket{x|x'+a}\braket{x'|0}dx'\\
        \psi(x)=\int\delta(x'-(x-a))\braket{x'|0}dx'\\
        \psi(x)=\braket{x-a|0}
      \end{gather*}
      Plugging this into the equation given:
      \begin{gather*}
        \psi(x)=\braket{x-a|0}=\pi^{-1/4}x_0^{-1/2}\exp\left[ -\frac{1}{2}\left( \frac{x-a}{x_0} \right)^2 \right]
      \end{gather*}
      \item The probability is:
      \begin{gather*}
        \text{Probability}=\left| \int\braket{x'|0}*\braket{x'|0}dx' \right|^2\\
        \text{Probability}=\left| \int\left( \pi^{-1/4}x_0^{-1/2}\exp\left[ -\frac{1}{2}\left( \frac{x'}{x_0} \right)^2 \right]\right)^2\right|^2\\
        \text{Probability}=-\frac{h e^{-\frac{m x \omega }{h}}}{\sqrt{\pi } m \omega  \sqrt{\frac{h}{m \omega }}}
      \end{gather*}
      Which doesn not change for $t>0$
    \end{enumerate}
    \item[2.16]
    \begin{enumerate}
      \item Starting by solving for $x$ and $p$:
      \begin{gather*}
        x=\sqrt{\frac{\hbar}{2m\omega}}(a+a^{\dagger})\\
        p=-\sqrt{\frac{\hbar m\omega}{2}}(a-a^{\dagger})
      \end{gather*}
      Solving for $\braket{m|x|n}$:
      \begin{gather*}
        \braket{m|x|n}=\sqrt{\frac{\hbar}{2m\omega}}\braket{m|a+a^{\dagger}|n}\\
        \braket{m|x|n}=\sqrt{\frac{\hbar}{2m\omega}}\braket{m|}\left(\sqrt{n}\ket{n-1}+\sqrt{n+1}\ket{n+1}  \right)\\
        \braket{m|x|n}=\sqrt{\frac{\hbar}{2m\omega}}\left( \sqrt{n}\delta_{m,n-1}+\sqrt{n+1}\delta_{m,n+1}\right)
      \end{gather*}
      Solving for $\braket{m|p|n}$:
      \begin{gather*}
        \braket{m|x|n}=-\sqrt{\frac{\hbar m\omega}{2}}\braket{m|a-a^{\dagger}|n}\\
        \braket{m|x|n}=-\sqrt{\frac{\hbar m\omega}{2}}\braket{m|}\left(\sqrt{n}\ket{n-1}-\sqrt{n+1}\ket{n+1}  \right)\\
        \braket{m|x|n}=-\sqrt{\frac{\hbar m\omega}{2}}\left( \sqrt{n}\delta_{m,n-1}-\sqrt{n+1}\delta_{m,n+1}\right)
      \end{gather*}
      Solving for $\braket{m|\{x,p\}|n}$, using $\{x,p\}=i\hbar(a^{\dagger}^2-a^2)$:
      \begin{gather*}
        \braket{m|x|n}=i\hbar\left(\sqrt{(n+1)(n+2)}\delta_{m,n+2}-\sqrt{n(n-1)}\delta_{m,n-2}\right)
      \end{gather*}
      Solving for $\braket{m|x^2|n}$:
      \begin{gather*}
        \braket{m|x^2|n}=\braket{m|\left(\sqrt{\frac{\hbar}{2m\omega}}(a+a^{\dagger})\right)^2|n}
      \end{gather*}
      Solving for $\braket{m|p^2|n}$:
      \begin{gather*}
        \braket{m|p^2|n}=\braket{m|\left(\sqrt{\frac{\hbar m\omega}{2}}(a-a^{\dagger})\right)^2|n}
      \end{gather*}
      \item[2.19]
      \begin{enumerate}
        \item
        \item
        \item
      \end{enumerate}

    \end{enumerate}
  \end{enumerate}

\end{document}