\documentclass[english]{article}
\usepackage{multicol}
\usepackage{physics}
\usepackage[margin=.75in]{geometry}
\begin{document}
\begin{multicols*}{2}
\textbf{Johannes Byle}\\

\noindent
\textbf{2.2}\\
$$\hat{P}_+=\ket{+z}\bra{+z}$$
$$\hat{P}_+^{\dag}=(\ket{+z})^{\dag}(\bra{+z})^{\dag}=\ket{+z}\bra{+z}$$
$$\hat{P}_+^2\Psi=\lambda^2\Psi=\hat{P}_+\Psi=\lambda\Psi$$
$$\lambda^2=\lambda$$
$$\lambda=0,1$$
\noindent
\textbf{2.4}\\
$$\bra{+y}\ket{+x}=\bra{+y}\ket{+z}\bra{+z}\ket{+x}+$$$$\bra{+y}\ket{-z}\bra{-z}\ket{+x}$$
$$\bra{+y}\ket{+x}=\frac{1}{\sqrt{2}}\frac{1}{\sqrt{2}}-\frac{i}{\sqrt{2}}\frac{1}{\sqrt{2}}$$
$$\bra{-y}\ket{+x}=\bra{-y}\ket{+z}\bra{+z}\ket{+x}+$$$$\bra{-y}\ket{-z}\bra{-z}\ket{+x}$$
$$\bra{-y}\ket{+x}=\frac{1}{\sqrt{2}}\frac{1}{\sqrt{2}}+\frac{i}{\sqrt{2}}\frac{1}{\sqrt{2}}$$
\[
\ket{+x}=\frac{1}{2}
\begin{bmatrix}
1-i\\
1+i
\end{bmatrix}
\]
$$\bra{+y}\ket{-x}=\bra{+y}\ket{+z}\bra{+z}\ket{-x}+$$$$\bra{+y}\ket{-z}\bra{-z}\ket{-x}$$
$$\bra{+y}\ket{-x}=\frac{1}{\sqrt{2}}\frac{1}{\sqrt{2}}-\frac{i}{\sqrt{2}}\frac{1}{\sqrt{2}}$$
$$\bra{-y}\ket{-x}=\bra{-y}\ket{+z}\bra{+z}\ket{-x}+$$$$\bra{-y}\ket{-z}\bra{-z}\ket{-x}$$
$$\bra{-y}\ket{-x}=\frac{1}{\sqrt{2}}\frac{1}{\sqrt{2}}+\frac{i}{\sqrt{2}}\frac{1}{\sqrt{2}}$$
\[
\ket{-x}=\frac{1}{2}
\begin{bmatrix}
1-i\\
1+i
\end{bmatrix}
\]
\noindent
\textbf{2.9}\\
\[
\begin{bmatrix}
1&2\\
3&4
\end{bmatrix}
^\dag
\begin{bmatrix}
5&7\\
6&8
\end{bmatrix}
^\dag
=
\begin{bmatrix}
5&21\\
12&31
\end{bmatrix}
\]

\[
\left(
\begin{bmatrix}
1&2\\
3&4
\end{bmatrix}
\begin{bmatrix}
5&7\\
6&8
\end{bmatrix}
\right)^\dag
=
\begin{bmatrix}
5&21\\
12&31
\end{bmatrix}
\]
\noindent
\textbf{2.11}\\
\[
\ket{\psi}=\frac{1}{\sqrt{2}}\frac{1}{\sqrt{3}}
\begin{bmatrix}
1\\
\sqrt{2}
\end{bmatrix}
\]
$$\langle S_x\rangle=\left(\frac{1}{\sqrt{2}\sqrt{3}}\right)^2\left(1+\sqrt{2}\right)\approx0.40$$
\noindent
\textbf{2.12}\\
\textbf{a)} $$\left(\frac{i}{\sqrt{3}}\right)^2=\frac{1}{3}$$
\textbf{b)} $$-\frac{2}{3}\sin\theta\ket{x}+\frac{i}{\sqrt{3}}\cos\theta\ket{y}$$
$$\lvert\bra{y'}\ket{\psi}\rvert^2=\frac{2}{3}\sin\theta\ket{x}+\frac{1}{3}\cos\theta\ket{y}$$
\textbf{c)} $$\ket{R}=\frac{1}{\sqrt{2}}\left(\ket{x}+i\ket{y}\right)=\frac{1}{\sqrt{3}}-\frac{1}{\sqrt{2}\sqrt{3}}$$
$$\ket{L}=1-\frac{1}{\sqrt{3}}+\frac{1}{\sqrt{2}\sqrt{3}}$$
Since $\ket{L}$ is larger it will spin in that direction\\
\textbf{d)} $$\left(\frac{1}{\sqrt{3}}\right)^2=\frac{1}{3}$$
$$-\frac{2}{3}\sin\theta\ket{x}+\frac{1}{\sqrt{3}}\cos\theta\ket{y}$$
$$\lvert\bra{y'}\ket{\psi}\rvert^2=\frac{2}{3}\sin\theta\ket{x}+\frac{1}{3}\cos\theta\ket{y}$$
$$\ket{R}=\frac{1}{\sqrt{2}}\left(\ket{x}+i\ket{y}\right)=\frac{1}{\sqrt{3}}+\frac{i}{\sqrt{2}\sqrt{3}}$$
$$\ket{L}=1-\frac{1}{\sqrt{3}}-\frac{i}{\sqrt{2}\sqrt{3}}$$
\end{multicols*}
\end{document}