\documentclass[english]{article}
\usepackage{multicol}
\usepackage{physics}
\usepackage[margin=.75in]{geometry}
\usepackage{amsmath}
\usepackage{verbatim}
\begin{document}
\textbf{Johannes Byle}\\
\noindent
\textbf{5.1}\\
\[
\hat{H}\rightarrow
\begin{bmatrix}
A/2 & 0 & 0 & 0\\
0 & -A/2 & A & 0\\
0 & A & -A/2 & 0\\
0 & 0 & 0 & A/2
\end{bmatrix}
,\ 
\omega_0\hat{S}_{1z}\rightarrow
\begin{bmatrix}
\tfrac{\hbar\omega_0}{2} & 0 & 0 & 0\\
0 & \tfrac{\hbar\omega_0}{2} & 0 & 0\\
0 & 0 & -\tfrac{\hbar\omega_0}{2} & 0\\
0 & 0 & 0 & -\tfrac{\hbar\omega_0}{2}
\end{bmatrix}
\]
\[
\hat{H}=\frac{2A}{\hbar^2}\hat{\vb{S}}_1\cdot\hat{\vb{S}}_2+\omega_0\hat{S}_{1z}\rightarrow
\begin{bmatrix}
\tfrac{A+\hbar\omega_0}{2} & 0 & 0 & 0\\
0 & \tfrac{-A+\hbar\omega_0}{2} & A & 0\\
0 & A & \tfrac{-A-\hbar\omega_0}{2} & 0\\
0 & 0 & 0 & \tfrac{A-\hbar\omega_0}{2}
\end{bmatrix}
\]
Eigenvalues:
\[
\det
\begin{bmatrix}
\tfrac{A+\hbar\omega_0}{2}-\lambda & 0 & 0 & 0\\
0 & \tfrac{-A+\hbar\omega_0}{2}-\lambda & A & 0\\
0 & A & \tfrac{-A-\hbar\omega_0}{2}-\lambda & 0\\
0 & 0 & 0 & \tfrac{A-\hbar\omega_0}{2}-\lambda
\end{bmatrix}
=- \frac{3 A^{4}}{16} + A^{3} \lambda + \frac{A^{2} \hbar\omega_0^{2}}{8} - \frac{3 A^{2} \lambda^{2}}{2} + \frac{\hbar\omega_0^{4}}{16} - \frac{\hbar\omega_0^{2} \lambda^{2}}{2} + \lambda^{4}
\]
$$\lambda = - \frac{A}{2} \pm \frac{\sqrt{4 A^{2} + \hbar\omega_0^{2}}}{2}, \  \frac{A}{2} \pm \frac{\hbar\omega_0}{2}$$
\begin{multicols}{2}
Assuming $(1+x)^n\approx1+nx$ and $A\gg\hbar\omega_0$:
$$\lambda=\frac{1}{2}\left(-A\pm\sqrt{4 A^{2} + \hbar\omega_0^{2}}\right)$$
$$\lambda=\frac{1}{2}\left(-A\pm A\sqrt{1 + \frac{\hbar\omega_0^{2}}{4A^2}}\right)$$
$$\lambda=\frac{A}{2} \pm \frac{\hbar\omega_0}{2},\ \frac{1}{2}\left(-A\pm A + \frac{\hbar\omega_0^{2}}{4A}\right)$$
Assuming $(1+x)^n\approx1+nx$ and $A\ll\hbar\omega_0$:
$$\lambda=\frac{1}{2}\left(-A\pm\sqrt{4 A^{2} + \hbar\omega_0^{2}}\right)$$
$$\lambda=\frac{1}{2}\left(-A\pm\hbar\omega_0\sqrt{\frac{4A^{2}}{\hbar\omega_0^2} + 1}\right)$$
$$\lambda=\frac{A}{2} \pm \frac{\hbar\omega_0}{2},\ \frac{1}{2}\left(-A\pm\hbar\omega_0\right)$$
\end{multicols}
\noindent
\textbf{5.6}\\
\[
\hat{H}\rightarrow
\begin{bmatrix}
A/2 & 0 & 0 & 0\\
0 & -A/2 & A & 0\\
0 & A & -A/2 & 0\\
0 & 0 & 0 & A/2
\end{bmatrix}
,\ 
\omega_0\left(\hat{S}_{1z}-\hat{S}_{2z}\right)\rightarrow
\begin{bmatrix}
0 & 0 & 0 & 0\\
0 & \hbar\omega_0 & 0 & 0\\
0 & 0 & -\hbar\omega_0 & 0\\
0 & 0 & 0 & 0
\end{bmatrix}
\]
\[
\hat{H}=\frac{2A}{\hbar^2}\hat{\vb{S}}_1\cdot\hat{\vb{S}}_2+\omega_0\left(\hat{S}_{1z}-\hat{S}_{2z}\right)\rightarrow
\begin{bmatrix}
A/2-\lambda & 0 & 0 & 0\\
0 & -A/2+\hbar\omega_0-\lambda & A & 0\\
0 & A & -A/2-\hbar\omega_0-\lambda & 0\\
0 & 0 & 0 & A/2-\lambda
\end{bmatrix}
\]
Eigenvalues:
\[
\det
\begin{bmatrix}
A/2-\lambda & 0 & 0 & 0\\
0 & -A/2+\hbar\omega_0-\lambda & A & 0\\
0 & A & -A/2-\hbar\omega_0-\lambda & 0\\
0 & 0 & 0 & A/2-\lambda
\end{bmatrix}
=- \frac{3 A^{4}}{16} + A^{3} \lambda - \frac{A^{2} \hbar\omega_0^{2}}{4} - \frac{3 A^{2} \lambda^{2}}{2} + A \hbar\omega_0^{2} \lambda - \hbar\omega_0^{2} \lambda^{2} + \lambda^{4}
\]
$$\lambda =  \frac{A}{2}, \  - \frac{A}{2} - \sqrt{A^{2} + \hbar\omega_0^{2}}, \  - \frac{A}{2} + \sqrt{A^{2} + \hbar\omega_0^{2}}$$
\begin{comment}
$$\ket{0,0}=\frac{1}{\sqrt{2}}\ket{+\vb{z},-\vb{z}}-\frac{1}{\sqrt{2}}\ket{-\vb{z},+\vb{z}}$$
$$\ket{+\vb{n}}=\cos\frac{\theta}{2}\ket{+\vb{z}}+e^{i\phi}\sin\frac{\theta}{2}\ket{-\vb{z}}$$
$$\ket{-\vb{n}}=\sin\frac{\theta}{2}\ket{+\vb{z}}-e^{i\phi}\cos\frac{\theta}{2}\ket{-\vb{z}}$$
$$\ket{0,0}=\frac{1}{\sqrt{2}}\left(\cos\frac{\theta}{2}\ket{+\vb{n}}+\sin\frac{\theta}{2}\ket{-\vb{n}}\right)\left(e^{i\phi}\sin\frac{\theta}{2}\ket{+\vb{n}}-e^{i\phi}\cos\frac{\theta}{2}\ket{-\vb{n}}\right)$$$$- \frac{1}{\sqrt{2}}\left(e^{i\phi}\sin\frac{\theta}{2}\ket{+\vb{n}}-e^{i\phi}\cos\frac{\theta}{2}\ket{-\vb{n}}\right)\left(\cos\frac{\theta}{2}\ket{+\vb{n}}+\sin\frac{\theta}{2}\ket{-\vb{n}}\right)$$
\[
\ket{0,0}=\frac{1}{\sqrt{2}}\left(
\begin{bmatrix}
\cos\tfrac{\theta}{2}e^{i\phi}\sin\tfrac{\theta}{2}\ket{+\vb{n},+\vb{n}} & -e^{i\phi}\cos^2\tfrac{\theta}{2}\ket{+\vb{n},-\vb{n}}\\
e^{i\phi}\sin^2\tfrac{\theta}{2}\ket{-\vb{n},+\vb{n}} & -\sin\tfrac{\theta}{2}e^{i\phi}\cos\tfrac{\theta}{2}\ket{-\vb{n},-\vb{n}}
\end{bmatrix}
-
\begin{bmatrix}
\cos\tfrac{\theta}{2}e^{i\phi}\sin\tfrac{\theta}{2}\ket{+\vb{n},+\vb{n}} & e^{i\phi}\sin^2\tfrac{\theta}{2}\ket{+\vb{n},-\vb{n}}\\
-e^{i\phi}\cos^2\tfrac{\theta}{2}\ket{-\vb{n},+\vb{n}} & -\sin\tfrac{\theta}{2}e^{i\phi}\cos\tfrac{\theta}{2}\ket{-\vb{n},-\vb{n}}
\end{bmatrix}
\right)
\]
\[
\ket{0,0}=\frac{1}{\sqrt{2}}
\begin{bmatrix}
0 & -e^{i\phi}\ket{+\vb{n},-\vb{n}}\\
e^{i\phi}\ket{-\vb{n},+\vb{n}} & 0
\end{bmatrix}
=\frac{e^{i\phi}}{\sqrt{2}}\ket{-\vb{n},+\vb{n}}-\frac{e^{i\phi}}{\sqrt{2}}\ket{+\vb{n},-\vb{n}}
\]
\end{comment}
\noindent
\textbf{5.7}\\
$$\ket{\tfrac{3}{2},\tfrac{3}{2}},\ \ket{\tfrac{3}{2},\tfrac{1}{2}},\ \ket{\tfrac{3}{2},-\tfrac{1}{2}},\ \ket{\tfrac{3}{2},-\tfrac{3}{2}}$$
\noindent
\textbf{5.10}\\
$$\ket{\psi}=\frac{1}{\sqrt{2}}\ket{x,x}+\frac{1}{\sqrt{2}}\ket{y,}$$
$$P\left(+\vb{a};+\vb{b}\right)=\left|\bra{+\vb{b}}\ket{+\vb{a}}\right|^2=\frac{1}{2}\sin^2 \frac{\theta}{2}$$
$$P\left(-\vb{a};+\vb{b}\right)=\left|\bra{-\vb{a}}\ket{+\vb{b}}\right|^2=\frac{1}{2}\cos^2 \frac{\theta}{2}$$
$$E\left(\vb{a},\vb{b}\right)=P_{++}\left(\vb{a},\vb{b}\right)+P_{--}\left(\vb{a},\vb{b}\right)-P_{+-}\left(\vb{a},\vb{b}\right)-P_{-+}\left(\vb{a},\vb{b}\right)$$
$$E\left(\vb{a},\vb{b}\right)=\sin^2\frac{\theta}{2}-\cos^2\frac{\theta}{2}=\cos\theta$$
\end{document}
